
$$
\frac{\partial h_{i}}{\partial p_{i}} = \frac{\partial x_{i}}{\partial p_{i}} + \frac{\partial x_{i}}{\partial m}\times \frac{\partial e}{\partial p_{i}}
$$
$$

\frac{\partial x_{i}}{\partial p_{i}} = \frac{\partial h_{i}}{\partial p_{i}} - \frac{\partial x_{i}}{\partial m}\times \frac{\partial e}{\partial p_{i}}
$$

$$
\begin{align*}
\end{align*}
$$
$$
\begin{align*}


e(p, u)&=p\cdot h(p,u) \\
&=p_{1}h_{1}(p_{1},\ p_{2},\ u) + p_{2}h_{2}(p_{1},\ p_{2},\ u) 

\\\\\\

\frac{\partial e}{\partial p_{1}} &= 
p_{1}h_{1}(p_{1},\ p_{2},\ u)+
p_{1}\frac{\partial h_{1}(p_{1},\ p_{2},\ u)}{\partial p_{1}}+
p_{2} \frac{\partial h_{2}(p_{1},\ p_{2},\ u)}{\partial p_{1}} \\\\
&= p_{1}h_{1}(p_{1},\ p_{2},\ u) + \sum\limits_{j}{p_{j}\frac{\partial h_{j}(p_{1},\ p_{2} ,\ u)}{\partial p_{1}}}






\end{align*}
$$

$$\frac{\partial e(p, u)}{\partial p_{1}}= h_{1}(p_{1},\ p_{2},\ u)$$